examples/knot_isotopy.lean
@@ -1,0 +1,140 @@
+import tidy.tidy
+
+inductive slice 
+| pos : ℕ → slice 
+| neg : ℕ → slice 
+| cup : ℕ → slice 
+| cap : ℕ → slice
+
+open slice
+
+inductive diagram
+| nil
+| cons : slice → diagram → diagram
+
+infixr ` ~~ `:80 := diagram.cons
+notation `t[` l:(foldr `, ` (h t, diagram.cons h t) diagram.nil `]`) := l
+
+
+
+namespace isotopy
+variable (d : diagram)
+axiom commute_pos_pos (n m) (h : n ≥ m + 2) : (pos n) ~~ (pos m) ~~ d = (pos m) ~~ (pos n) ~~ d
+axiom commute_pos_neg (n m) (h : n ≥ m + 2) : (pos n) ~~ (neg m) ~~ d = (neg m) ~~ (pos n) ~~ d
+axiom commute_neg_pos (n m) (h : n ≥ m + 2) : (neg n) ~~ (pos m) ~~ d = (pos m) ~~ (neg n) ~~ d
+axiom commute_neg_neg (n m) (h : n ≥ m + 2) : (neg n) ~~ (neg m) ~~ d = (neg m) ~~ (neg n) ~~ d
+
+axiom commute_cup_pos (n m) (h : n ≥ m + 2) : (cup n) ~~ (pos m) ~~ d = (pos m) ~~ (cup n) ~~ d 
+axiom commute_cup_neg (n m) (h : n ≥ m + 2) : (cup n) ~~ (neg m) ~~ d = (neg m) ~~ (cup n) ~~ d 
+axiom commute_cap_pos (n m) (h : n ≥ m + 2) : (cap n) ~~ (pos m) ~~ d = (pos m) ~~ (cap n) ~~ d 
+axiom commute_cap_neg (n m) (h : n ≥ m + 2) : (cap n) ~~ (neg m) ~~ d = (neg m) ~~ (cap n) ~~ d 
+
+axiom commute_pos_cup (n m) (h : n ≥ m)     : (pos n) ~~ (cup m) ~~ d = (cup m) ~~ (pos (n+2)) ~~ d 
+axiom commute_pos_cap (n m) (h : n ≥ m + 2) : (pos n) ~~ (cap m) ~~ d = (cap m) ~~ (pos (n-2)) ~~ d 
+axiom commute_neg_cup (n m) (h : n ≥ m)     : (neg n) ~~ (cup m) ~~ d = (cup m) ~~ (neg (n+2)) ~~ d 
+axiom commute_neg_cap (n m) (h : n ≥ m + 2) : (neg n) ~~ (cap m) ~~ d = (cap m) ~~ (neg (n-2)) ~~ d 
+
+axiom commute_cup_cup (n m) (h : n ≥ m)     : (cup n) ~~ (cup m) ~~ d = (cup m) ~~ (cup (n+2)) ~~ d 
+axiom commute_cup_cap (n m) (h : n ≥ m + 2) : (cup n) ~~ (cap m) ~~ d = (cap m) ~~ (cup (n-2)) ~~ d 
+axiom commute_cap_cup (n m) (h : n ≥ m)     : (cap n) ~~ (cup m) ~~ d = (cup m) ~~ (cap (n+2)) ~~ d 
+axiom commute_cap_cap (n m) (h : n ≥ m + 2) : (cap n) ~~ (cap m) ~~ d = (cap m) ~~ (cap (n-2)) ~~ d 
+
+axiom zigzag_left (n : ℕ) : (cup n) ~~ (cap (n+1)) ~~ d = d  
+axiom zigzag_right (n : ℕ) : (cup (n+1)) ~~ (cap n) ~~ d = d
+
+axiom R2_east (n : ℕ) : (neg n) ~~ (pos n) ~~ d = d
+axiom R2_west (n : ℕ) : (pos n) ~~ (neg n) ~~ d = d
+-- axiom R2_north (n : ℕ) : (cup (n+1)) ~~ (pos n) ~~ (neg (n+2)) ~~ cup(n+1) ~~ d = (cap n) ~~ (cup n) ~~ d
+-- axiom R2_south (n : ℕ) : (cup (n+1)) ~~ (neg n) ~~ (pos (n+2)) ~~ cup(n+1) ~~ d = (cap n) ~~ (cup n) ~~ d
+
+axiom R1_pos_east (n : ℕ) : (cup (n+1)) ~~ (pos n) ~~ (cap (n+1)) ~~ d = d
+axiom R1_neg_east (n : ℕ) : (cup (n+1)) ~~ (neg n) ~~ (cap (n+1)) ~~ d = d
+axiom R1_pos_west (n : ℕ) : (cup n) ~~ (pos (n+1)) ~~ (cap n) ~~ d = d
+axiom R1_neg_west (n : ℕ) : (cup n) ~~ (neg (n+1)) ~~ (cap n) ~~ d = d
+axiom R1_pos_north (n : ℕ) : (pos n) ~~ (cap n) ~~ d = (cap n) ~~ d
+axiom R1_neg_north (n : ℕ) : (neg n) ~~ (cap n) ~~ d = (cap n) ~~ d
+axiom R1_pos_south (n : ℕ) : (cup n) ~~ (pos n) ~~ d = (cup n) ~~ d
+axiom R1_neg_south (n : ℕ) : (cup n) ~~ (neg n) ~~ d = (cup n) ~~ d
+
+axiom R3_pos_pos_pos (n : ℕ) : (pos n) ~~ (pos (n+1)) ~~ (pos n) ~~ d = (pos (n+1)) ~~ (pos n) ~~ (pos (n+1)) ~~ d
+axiom R3_pos_pos_neg (n : ℕ) : (pos n) ~~ (pos (n+1)) ~~ (neg n) ~~ d = (neg (n+1)) ~~ (pos n) ~~ (pos (n+1)) ~~ d
+axiom R3_pos_neg_neg (n : ℕ) : (pos n) ~~ (neg (n+1)) ~~ (neg n) ~~ d = (neg (n+1)) ~~ (neg n) ~~ (pos (n+1)) ~~ d
+axiom R3_neg_pos_pos (n : ℕ) : (neg n) ~~ (pos (n+1)) ~~ (pos n) ~~ d = (pos (n+1)) ~~ (pos n) ~~ (neg (n+1)) ~~ d
+axiom R3_neg_neg_pos (n : ℕ) : (neg n) ~~ (neg (n+1)) ~~ (pos n) ~~ d = (pos (n+1)) ~~ (neg n) ~~ (neg (n+1)) ~~ d
+axiom R3_neg_neg_neg (n : ℕ) : (neg n) ~~ (neg (n+1)) ~~ (neg n) ~~ d = (neg (n+1)) ~~ (neg n) ~~ (neg (n+1)) ~~ d
+
+axiom cap_over  (n : ℕ) : (pos n) ~~ (cap (n+1)) ~~ d = (neg (n+1)) ~~ (cap n) ~~ d
+axiom cap_under (n : ℕ) : (neg n) ~~ (cap (n+1)) ~~ d = (pos (n+1)) ~~ (cap n) ~~ d
+axiom cup_over  (n : ℕ) : (cup (n+1)) ~~ (neg n) ~~ d = (cup n) ~~ (pos (n+1)) ~~ d
+axiom cup_under (n : ℕ) : (cup (n+1)) ~~ (pos n) ~~ d = (cup n) ~~ (neg (n+1)) ~~ d
+
+-- axiom rotate_pos_clockwise   (n : ℕ) : (cup n) ~~ (pos (n+1)) ~~ (cap (n+2)) ~~ d = (neg n) ~~ d
+-- axiom rotate_neg_clockwise   (n : ℕ) : (cup n) ~~ (neg (n+1)) ~~ (cap (n+2)) ~~ d = (pos n) ~~ d
+-- axiom rotate_pos_widdershins (n : ℕ) : (cup (n+2)) ~~ (pos (n+1)) ~~ (cap n) ~~ d = (neg n) ~~ d
+-- axiom rotate_neg_widdershins (n : ℕ) : (cup (n+2)) ~~ (neg (n+1)) ~~ (cap n) ~~ d = (pos n) ~~ d
+
+attribute [search] commute_pos_pos commute_pos_neg commute_neg_pos commute_neg_neg
+attribute [search] commute_cup_pos commute_cup_neg commute_cap_pos commute_cap_neg
+attribute [search] commute_pos_cup commute_pos_cap commute_neg_cup commute_neg_cap
+attribute [search] commute_cup_cup commute_cup_cap commute_cap_cup commute_cap_cap
+attribute [search] zigzag_left zigzag_right
+attribute [search] cap_over cap_under cup_over cup_under
+attribute [search] R1_pos_east R1_neg_east R1_pos_west R1_neg_west R1_pos_north R1_neg_north R1_pos_south R1_neg_south
+attribute [search] R2_east R2_west -- R2_north R2_south
+attribute [search] R3_pos_pos_pos R3_pos_pos_neg R3_pos_neg_neg R3_neg_pos_pos R3_neg_neg_pos R3_neg_neg_neg 
+-- attribute [search] rotate_pos_clockwise rotate_neg_clockwise rotate_pos_widdershins rotate_neg_widdershins
+
+end isotopy
+
+namespace norm_num
+open tactic
+
+meta def derive' : expr → tactic (expr × expr) | e :=
+do (_, e', pr) ←
+    ext_simplify_core () {} simp_lemmas.mk (λ _, failed) (λ _ _ _ _ _, failed)
+      (λ _ _ _ _ e,
+        do (new_e, pr) ← derive1 derive' e,
+           guard (¬ new_e =ₐ e),
+           return ((), new_e, some pr, tt))
+      `eq e,
+    return (e', pr)
+end norm_num
+
+open isotopy
+open tactic
+
+meta def isotopy := `[rewrite_search_using [`search] { discharger := `[norm_num], trace_result := tt }]
+
+-- lemma commute_1 : t[pos 0, neg 2, pos 4] = t[pos 4, neg 2, pos 0] := by isotopy
+-- lemma commute_2 : t[cup 0, pos 2] = t[pos 0, cup 0] := by isotopy
+-- lemma commute_3 : t[cup 2, cap 0] = t[cup 0, cap 2] := by isotopy
+-- lemma bulge : t[cup 1, cap 0, cup 0, cap 1] = t[] := by isotopy
+
+-- lemma R2_south' : [cup 1, pos 0, neg 2, cap 1] = [cup 0, neg 1, neg 2, cap 1] := by isotopy
+
+lemma R2_south : t[cup 1, pos 0, neg 2, cap 1] = t[cap 0, cup 0] := 
+begin
+(do `(%%lhs = %%rhs) ← target, all_rewrites (`(cup_under),ff) ff lhs { discharger := `[norm_num1], simplifier := norm_num.derive } >>= trace),
+
+-- rewrite_search_using [`search] { discharger := `[norm_num], simplifier := norm_num.derive, trace := tt },
+-- rw cup_under, 
+-- isotopy,
+-- rw ← cap_over,
+-- rw R2_east,
+-- rw commute_cap_cup,
+-- norm_num
+end
+-- by isotopy
+
+lemma twists : [cup 0, cup 2, pos 0, pos 2, cap 1, cap 0] = [cup 0, cap 0] := by isotopy
+-- begin
+-- rw cup_pos_commute,
+-- rw R1_pos_south,
+-- rw R1_pos_south,
+-- rw zigzag_right,
+-- norm_num
+-- end
+
+lemma rotate : [cup 0, pos 1, cap 2] = [neg 0] := by isotopy
+
+-- lemma recognise_trefoil : [cup 0, cup 1, pos 0, pos 0, pos 0, cap 1, cap 0] = [cup 0, cup 2, neg 1, pos 0, pos 2, cap 1, cap 0] := by isotopy
